PyLevelLang/src/PyLevelLang/Examples.v
@@ -1,0 +1,79 @@
+Require Import PyLevelLang.Language.
+Require Import PyLevelLang.Elaborate.
+Require Import PyLevelLang.Interpret.
+Require Import coqutil.Map.Interface coqutil.Map.SortedListString.
+Require Import coqutil.Datatypes.Result.
+Import ResultMonadNotations.
+
+Section Examples.
+  Instance tenv : map.map string (type * bool) := SortedListString.map _.
+  Instance tenv_ok : map.ok tenv := SortedListString.ok _.
+  
+  Instance locals : map.map string {t & interp_type t} := SortedListString.map _.
+  Instance locals_ok : map.ok locals := SortedListString.ok _.
+
+  Definition elaborate_interpret (p : pexpr) : result {t & interp_type t} :=
+    match elaborate map.empty p with
+    | Success v => Success (existT _ _ (interp_expr map.empty (projT2 v)))
+    | Failure e => Failure e
+    end.
+
+  Local Open Scope Z_scope.
+  Local Open Scope string_scope.
+
+  Definition ex1 : pexpr :=
+    PEBinop POCons (PEConst (CInt 1))
+      (PEBinop POCons (PEConst (CInt 2))
+        (PEBinop POCons (PEConst (CInt 3))
+          (PESingleton (PEConst (CInt 4))))).
+  Goal elaborate map.empty ex1 =
+    Success (existT _ _
+      (EBinop (OCons _) (EConst (CInt 1))
+        (EBinop (OCons _) (EConst (CInt 2))
+          (EBinop (OCons _) (EConst (CInt 3))
+            (EBinop (OCons _) (EConst (CInt 4))
+              (EConst (CNil _))))))).
+  reflexivity. Qed.
+  Goal elaborate_interpret ex1 = Success (existT _ (TList TInt) (1 ::  2 :: 3 :: 4 :: nil)).
+  reflexivity. Qed.
+
+  Definition ex2 : pexpr :=
+    PEBinop POCons (PEConst (CString "a")) (
+      PEBinop POCons (PEConst (CInt 2)) (
+        PEBinop POCons (PEConst (CInt 3)) (
+          PESingleton (PEConst (CInt 4))))).
+  Goal elaborate map.empty ex2 = error:("POCons with mismatched types").
+  reflexivity. Qed.
+  Goal elaborate_interpret ex2 = error:("POCons with mismatched types").
+  reflexivity. Qed.
+
+  Definition ex3 : pexpr :=
+    PEUnop POFst (PELet "x"
+      (PEConst (CInt 42)) (PEBinop POPair (PEVar "x") (PEVar "x"))).
+  Goal elaborate map.empty ex3 =
+    Success (existT _ _
+      (EUnop (OFst _ _) (ELet "x"
+        (EConst (CInt 42)) (EBinop (OPair _ _) (EVar TInt "x") (EVar TInt "x"))))).
+  reflexivity. Qed.
+  Goal elaborate_interpret ex3 = Success (existT _ TInt 42).
+  reflexivity. Qed.
+
+  Definition ex4 : pexpr :=
+    PEUnop POFst (PELet "x"
+      (PEConst (CInt 42)) (PEBinop POPair (PEVar "x") (PEVar "y"))).
+  Goal elaborate map.empty ex4 = error:("PEVar with undefined variable").
+  reflexivity. Qed.
+  Goal elaborate_interpret ex4 = error:("PEVar with undefined variable").
+  reflexivity. Qed.
+
+  Definition ex5 : pexpr :=
+    PEBinop POPair (PEConst (CInt 42))
+      (PEBinop POPair (PEConst (CBool true)) (PEConst (CString "hello"))).
+  Goal elaborate map.empty ex5 =
+    Success (existT _ _
+      (EBinop (OPair _ _) (EConst (CInt 42))
+        (EBinop (OPair _ _) (EConst (CBool true)) (EConst (CString "hello"))))).
+  reflexivity. Qed.
+  Goal elaborate_interpret ex5 = Success (existT _ (TPair TInt (TPair TBool TString)) (42, (true, "hello"))).
+  reflexivity. Qed.
+End Examples.
